\documentclass[utf8]{ctexart}
\usepackage{graphicx}
\usepackage{amsmath}
\title{线代作业6}
\author{郑子诺，物理41}
\date{\today}
\begin{document}
\maketitle
\noindent1.\\
(1)
\[\begin{vmatrix}
	1&2&3&4\\
	0&1&0&2\\
	1&0&1&1\\
	2&3&0&1
\end{vmatrix}
=\begin{vmatrix}
	1&0&2\\
	0&1&1\\
	3&0&1
\end{vmatrix}+
\begin{vmatrix}
	2&3&4\\
	1&0&2\\
	3&0&1
\end{vmatrix}
-2\begin{vmatrix}
	2&3&4\\
	1&0&2\\
	0&1&1
\end{vmatrix}
=16\]
(2)
\begin{align*}
	\begin{vmatrix}
		1&0&0&0&1\\
		0&1&0&1&0\\
		0&0&1&0&1\\
		1&1&1&1&1\\
		2&3&4&5&6
	\end{vmatrix}
	&=\begin{vmatrix}
		1&0&1&0\\
		0&1&0&1\\
		1&1&1&1\\
		3&4&5&6
	\end{vmatrix}
	+\begin{vmatrix}
		0&1&0&1\\
		0&0&1&0\\
		1&1&1&1\\
		2&3&4&5
	\end{vmatrix}\\
	&=\begin{vmatrix}
		1&0&1\\
		1&1&1\\
		4&5&6
	\end{vmatrix}+\begin{vmatrix}
	0&1&1\\
	1&1&1\\
	3&4&6
	\end{vmatrix}-\begin{vmatrix}
	0&1&1\\
	1&1&1\\
	2&3&5
	\end{vmatrix}=2
\end{align*}
2.\\
\begin{align*}
	&\begin{vmatrix}
		1&1&0&0&\cdots&0\\
		-1&1&1&0&\cdots&0\\
		0&-1&1&1&\cdots&0\\
		\vdots&\vdots&\vdots&\vdots&\ddots&\vdots\\
		0&0&\cdots&-1&1&1\\
		0&0&\cdots&0&-1&1
	\end{vmatrix}\\
	&=\begin{vmatrix}
		1&1&0&\cdots&0\\
		-1&1&1&\cdots&0\\
		\vdots&\vdots&\vdots&\ddots&\vdots\\
		0&\cdots&-1&1&1\\
		0&\cdots&0&-1&1
	\end{vmatrix}-\begin{vmatrix}
	-1&1&0&\cdots&0\\
	0&1&1&\cdots&0\\
	\vdots&\vdots&\vdots&\ddots&\vdots\\
	0&\cdots&-1&1&1\\
	0&\cdots&0&-1&1
	\end{vmatrix}\\
	&=\begin{vmatrix}
		1&1&0&\cdots&0\\
		-1&1&1&\cdots&0\\
		\vdots&\vdots&\vdots&\ddots&\vdots\\
		0&\cdots&-1&1&1\\
		0&\cdots&0&-1&1
	\end{vmatrix}+\begin{vmatrix}
	1&1&\cdots&0\\
	\vdots&\vdots&\ddots&\vdots\\
	0&\cdots&1&1\\
	0&\cdots&-1&1
	\end{vmatrix}
\end{align*}
所以有
\[F_n=F_{n-1}+F_{n-2}\]
显然
\[F_1=1,F_2=2\]
3.\\
\begin{align*}
	\frac{d\det A}{dx}&=\sum\limits_{\sigma}sgn(\sigma)\frac{d}{dx}(a_{1\sigma(1)}a_{2\sigma(2)}\cdots a_{n\sigma(n)})\\
	&=\sum\limits_{\sigma}sgn(\sigma)\sum\limits_{i=1}^n\frac{da_{i\sigma(i)}}{dx}a_{1\sigma(1)}\cdots\widehat{a_{i\sigma(i)}}\cdots a_{n\sigma(n)}\\
	&=\sum\limits_{i=1}^n\sum\limits_{j=1}^n\frac{da_{ij}}{dx}\sum\limits_{\sigma'}sgn(\sigma'(1)\cdots j\cdots\sigma'(n))a_{1\sigma'(1)}\cdots\widehat{a_{ij}}\cdots a_{n\sigma'(n)}\\
	&=\sum\limits_{i=1}^n\sum\limits_{j=1}^n(-1)^{i-1}\frac{da_{ij}}{dx}\sum\limits_{\sigma'}sgn(j\sigma')a_{1\sigma'(1)}\cdots\widehat{a_{ij}}\cdots a_{n\sigma'(n)}\\
	&=\sum\limits_{i=1}^n\sum\limits_{j=1}^n(-1)^{i+j}\frac{da_{ij}}{dx}\sum\limits_{\sigma'}sgn(\sigma')a_{1\sigma'(1)}\cdots\widehat{a_{ij}}\cdots a_{n\sigma'(n)}\\
	&=\sum\limits_{i=1}^n\sum\limits_{j=1}^n(-1)^{i+j}\frac{da_{ij}}{dx}A_{ij}
\end{align*}
4.\\
(a)对于第一条式子，显然前$m\times m$个元素为$I_m$，我们有
\[1\le i\le m,m+1\le j\le m+n,c_{ij}=\sum\limits_{k=1}^{m+n}\delta_{ik}a_{k(j-m)}=a_{i(j-m)}\]
\[m+1\le i\le m+n,1\le j\le m,c_{ij}=\sum\limits_{k=1}^{m}-b_{(i-m)k}\delta_{kj}+\sum\limits_{k=m+1}^{m+n}\delta_{ik}b_{(k-m)j}=0\]
\[m+1\le i\le m+n,m+1\le j\le m+n,c_{ij}=\sum\limits_{k=1}^{m}-b_{(i-m)k}a_{k(j-m)}+\sum\limits_{k=m+1}^{m+n}\delta_{ik}\delta_{kj}=\delta_{ij}-(BA)_{(i-m)(j-m)}\]
所以
\[\begin{bmatrix}
	I_m&0\\
	-B&I_n
\end{bmatrix}
\begin{bmatrix}
	I_m&A\\
	B&I_n
\end{bmatrix}
=\begin{bmatrix}
	I_m&A\\
	0&I_n-BA
\end{bmatrix}\]
对于第二条式子，后面$n\times n$也是显然的，我们有
\[1\le i\le m,1\le j\le m,c_{ij}=\sum\limits_{k=1}^{m}\delta_{ik}\delta_{ij}+\sum\limits_{k=m+1}^{m+n}-a_{i(k-m)}b_{(k-m)j}=\delta_{ij}-(AB)_{ij}\]
\[1\le i\le m,m+1\le j\le m+n,c_{ij}=\sum\limits_{k=1}^{m}\delta_{ik}a_{k(j-m)}+\sum\limits_{k=m+1}^{m+n}-a_{i(k-m)}\delta_{kj}=0\]
\[m+1\le i\le m+n,1\le j\le m,c_{ij}=\sum\limits_{k=1}^{m+n}\delta_{ik}b_{(k-m)j}=b_{(i-m)j}\]
所以
\[\begin{bmatrix}
	I_m&-A\\
	0&I_n
\end{bmatrix}
\begin{bmatrix}
	I_m&A\\
	B&I_n
\end{bmatrix}
=\begin{bmatrix}
	I_m-AB&0\\
	B&I_n
\end{bmatrix}\]
(b)
\begin{align*}
	\det(I_m-AB)&=\det\begin{bmatrix}
		I_m-AB&0\\
		B&I_n
	\end{bmatrix}\\
	&=\det\begin{bmatrix}
		I_m&A\\
		B&I_n
	\end{bmatrix}\\
	&=\det\begin{bmatrix}
		I_m&A\\
		0&I_n-BA
	\end{bmatrix}\\
	&=\det(I_n-BA)
\end{align*}
(c)
\begin{align*}
	\begin{vmatrix}
		1+a_1b_1&a_1b_2&\cdots&a_1b_n\\
		a_2b_1&1+a_2b_2&\cdots&a_2b_n\\
		\vdots&\vdots&\ddots&\vdots\\
		a_nb_1&a_nb_2&\cdots&1+a_nb_n
	\end{vmatrix}=\det(I_n-BA)
\end{align*}
其中
\[B=\begin{bmatrix}
	b_1\\
	b_2\\
	\vdots\\
	b_n
\end{bmatrix},A=\begin{bmatrix}
-a_1&-a_2&\cdots&-a_n
\end{bmatrix}\]
所以
\begin{align*}
	\begin{vmatrix}
		1+a_1b_1&a_1b_2&\cdots&a_1b_n\\
		a_2b_1&1+a_2b_2&\cdots&a_2b_n\\
		\vdots&\vdots&\ddots&\vdots\\
		a_nb_1&a_nb_2&\cdots&1+a_nb_n
	\end{vmatrix}&=\det(I_n-BA)\\
	&=\det(1-AB)\\
	&=1+a_1b_1+a_2b_2+\cdots+a_nb_n
\end{align*}
\end{document}













