\documentclass[utf8]{ctexart}
\usepackage{graphicx}
\usepackage{amsmath}
\usepackage{braket}
\usepackage{amssymb}
\makeatletter
\newcommand{\rmnum}[1]{\romannumeral #1}
\newcommand{\Rmnum}[1]{\expandafter\@slowromancap\romannumeral #1@}
\makeatother
\title{费曼3作业6}
\author{郑子诺，物理41}
\date{\today}
\begin{document}
\maketitle
\noindent77.1\\
\begin{align*}
	i\hbar\dot{a}&=-\mu B\cos\theta a-\mu B\sin\theta e^{i\omega t}b\\
	i\hbar\dot{b}&=-\mu B\sin\theta e^{-i\omega t}a+\mu B\cos\theta b
\end{align*}
The zero order:
\begin{align*}
	i\hbar\dot{a_0}&=-\mu Ba_0\\
	i\hbar\dot{b_0}&=\mu Bb_0
\end{align*}
we have
\[a_0=e^{i\frac{\mu B}{\hbar}t},b_0=0\]
Then we consider the first order. We notice that the first equation has no first order.
\[i\hbar\dot{b}=-\mu B\sin\theta e^{-i\omega t}e^{i\frac{\mu B}{\hbar}t}+\mu Bb\]
we have
\[b=\frac{\frac{\mu B}{\hbar}\sin\theta}{\frac{2\mu B}{\hbar}-\omega}(e^{i(\frac{\mu B}{\hbar}-\omega)t}-e^{-i\frac{\mu B}{\hbar}t})\]
Obviously, $\omega$ must be $\dfrac{2\mu B}{\hbar}$ for resonance. Then we have
\[b=i\frac{\mu B}{\hbar}te^{-i\frac{\mu B}{\hbar}t}\sin\theta\]
\[P_{-z}=|b|^2=\frac{\mu^2B^2}{\hbar^2}t^2\sin^2\theta\]
77.2\\
Like 77.1, let $z$-axis along $B_0$, we have
\[a_0=0,b_0=e^{-i\frac{\mu B_0}{\hbar}t}\]
\[i\hbar\dot{a}=-\mu B_n(e^{i\omega t}+e^{-i\omega t})e^{i\frac{\mu B_0}{\hbar}t}-\mu B_0a\]
If $\omega\neq\frac{2\mu B_0}{\hbar},-\frac{2\mu B_0}{\hbar}$, we have
\[a=\frac{\frac{\mu B_n}{\hbar}}{\omega-\frac{2\mu B_0}{\hbar}}e^{i(\omega-\frac{\mu B_0}{\hbar})t}-\frac{\frac{\mu B_n}{\hbar}}{\omega+\frac{2\mu B_0}{\hbar}}e^{-i(\omega+\frac{\mu B_0}{\hbar})t}-\frac{\frac{4\mu^2 B_0B_n}{\hbar^2}}{\omega^2-\frac{4\mu^2 B_0^2}{\hbar^2}}e^{i\frac{\mu B_0}{\hbar}t}\]
\begin{align*}
	P_{||}&=|a|^2\\
	&=(\frac{\frac{\mu B_n}{\hbar}}{\omega-\frac{2\mu B_0}{\hbar}})^2+(\frac{\frac{\mu B_n}{\hbar}}{\omega+\frac{2\mu B_0}{\hbar}})^2+(\frac{\frac{4\mu^2 B_0B_n}{\hbar^2}}{\omega^2-\frac{4\mu^2 B_0^2}{\hbar^2}})^2\\
	&-\frac{\frac{2\mu^2 B_n^2}{\hbar^2}}{\omega^2-\frac{4\mu^2 B_0^2}{\hbar^2}}\cos2\omega t-2\frac{\frac{\mu B_n}{\hbar}}{\omega-\frac{2\mu B_0}{\hbar}}\frac{\frac{4\mu^2 B_0B_n}{\hbar^2}}{\omega^2-\frac{4\mu^2 B_0^2}{\hbar^2}}\cos(\omega-\frac{2\mu B_0}{\hbar})t\\
	&+2\frac{\frac{\mu B_n}{\hbar}}{\omega+\frac{2\mu B_0}{\hbar}}\frac{\frac{4\mu^2 B_0B_n}{\hbar^2}}{\omega^2-\frac{4\mu^2 B_0^2}{\hbar^2}}\cos(\omega+\frac{2\mu B_0}{\hbar})t
\end{align*}
If $\omega=\frac{2\mu B_0}{\hbar}\text{ or }-\frac{2\mu B_0}{\hbar}$, we have
\[a\approx i\frac{\mu B_n}{\hbar}te^{i\frac{\mu B_0}{\hbar}t}\]
\[P_{||}=|a|^2=\frac{\mu^2B_n^2}{\hbar^2}t^2\]
\end{document}























