\documentclass[utf8]{ctexart}
\usepackage{graphicx}
\usepackage{amsmath}
\usepackage{braket}
\usepackage{amssymb}
\usepackage{bm}
\usepackage{siunitx}
\usepackage{float}
\makeatletter
\newcommand{\rmnum}[1]{\romannumeral #1}
\newcommand{\Rmnum}[1]{\expandafter\@slowromancap\romannumeral #1@}
\makeatother
\title{费曼3作业10}
\author{郑子诺，物理41}
\date{\today}
\begin{document}
\maketitle
\noindent80.4\\
(a)Suppose $\beta=a+ib$, use $|\beta|^2+|1+\beta|^2=1$ we have
\[b^2=-a(1+a)\]
and we also have
\[\frac{\beta}{1+\beta}=\frac{a+ib}{1+a+ib}=\frac{a(1+a)+b^2+ib}{(1+a)^2+b^2}\]
and therefore
\[\mathrm{Re}\{\frac{\beta}{1+\beta}\}=\frac{a(1+a)+b^2}{(1+a)^2+b^2}=0\]
(b)Let $\dfrac{\beta}{1+\beta}=i\tan\eta$, we have
\[\beta=\frac{i\tan\eta}{1-i\tan\eta}=\frac{i\sin\eta}{\cos\eta-i\sin\eta}=i(\cos\eta+\sin\eta)\sin\eta=ie^{i\eta}\sin\eta\]
83.4\\
(a)Use the Schrodinger equation, we have
\[i\hbar(-\frac{\mathrm{d}a}{\mathrm{d}t}x^2-\frac{\mathrm{d}c}{\mathrm{d}t})=-\frac{\hbar^2}{2m}(4a^2x^2-2a)\]
and then
\[(i\hbar\frac{\mathrm{d}a}{\mathrm{d}t}-\frac{2\hbar^2}{m}a^2)x^2+i\hbar\frac{\mathrm{d}c}{\mathrm{d}t}+\frac{\hbar^2}{m}a=0\]
Because this equation should be correct for all $x$, we have
\[\frac{\mathrm{d}a}{\mathrm{d}t}=-\frac{2i\hbar}{m}a^2\]
and
\[\frac{1}{a(t)}=\frac{1}{a_0}+\frac{2i\hbar}{m}t\]
(b)Use the equation above, we also have
\[c(t)=\frac{1}{2}\ln(1+\frac{2i\hbar a_0}{m}t)+c_0\]
(c)We have
\[\mathrm{Re}\{a(t)\}=\frac{a_0}{1+\frac{4\hbar^2a_0^2}{m^2}t^2}\]
Let $\dfrac{1}{\sqrt{a_0}}=1\unit{\mathring{A}},t=1\unit{s}$, we have
\[d=\frac{1}{\sqrt{\mathrm{Re}\{a(t)\}}}=2.3\times 10^{6}\unit{m}\]
(d)We have
\[\phi(p)=\int_{-\infty}^{+\infty}\frac{1}{\sqrt{2\pi\hbar}}e^{-i\frac{p}{\hbar}x}\psi(x)\mathrm{d}x=\frac{K}{\sqrt{2a\hbar}}e^{-(\frac{p^2}{4a\hbar^2}+c)}\]
(e)We have
\[\Delta p=\sqrt{4\mathrm{Re}\{a(t)\}\hbar^2}=\sqrt{\frac{4a_0\hbar^2}{1+\frac{4\hbar^2a_0^2}{m^2}t^2}}\]
(f)Obviously we have
\[\frac{\mathrm{d}\frac{1}{\sqrt{a(t)}}}{\mathrm{d}t}=i\hbar\sqrt{a(t)}\]
Then
\[2|i\hbar\sqrt{a(t)}|=2\sqrt{|a(t)|}\hbar=\Delta p\]
\end{document}



















